Switch to abstract state

src/tls/EverCrypt.CRF.fst
@@ -9,8 +9,10 @@ module HS = FStar.HyperStack
 
 open FStar.HyperStack.ST
 
-/// migrate these 2 functions to no_extract LowStar.Buffer?
+/// Helpers
+/// -------
 ///
+/// migrate these 2 functions to no_extract LowStar.Buffer?
 assume val to_seq
   (#a:Type0)
   // (#rrel #rel:B.srel a)
@@ -38,6 +40,87 @@ assume val of_seq
     (fun h0 _ h1 ->
       B.modifies (B.loc_buffer b) h0 h1 /\
       B.as_seq h1 b == s)
+
+/// Implementing abstract types
+/// ---------------------------
+
+/// This is very finely tuned to avoid inference issues.
+type mstate a = a': Concrete.alg { a' == a } & p:B.pointer bytes {
+  B.(loc_disjoint (loc_addr_of_buffer p) (loc_region_only true Mem.tls_tables_region))
+}
+
+let state (a: Concrete.alg) =
+  if model then
+    mstate a
+  else
+    Concrete.state a
+
+// UGH!!!
+noextract inline_for_extraction
+let fst (#a: e_alg) (s: state (G.reveal a){model}):
+  Tot (a': Concrete.alg { G.reveal a == a' })
+=
+  if model then
+    let (| a, s |) = (s <: mstate (G.reveal a)) in
+    a
+  else
+    false_elim ()
+
+noextract inline_for_extraction
+let snd (#a: e_alg) (s: state (G.reveal a){model}):
+  Tot (p:B.pointer bytes {
+    B.(loc_disjoint (loc_addr_of_buffer p) (loc_region_only true Mem.tls_tables_region))
+  })
+=
+  if model then
+    let (| a, s |) = (s <: mstate (G.reveal a)) in
+    s
+  else
+    false_elim ()
+
+let freeable #a h (s:state a) =
+  if model then
+    let s: B.pointer bytes = snd #(G.hide a) s in
+    B.freeable s
+  else
+    Concrete.freeable #a h s
+
+let footprint #a h (s: state a) =
+  if model then
+    B.loc_addr_of_buffer (snd #(G.hide a) s)
+  else
+    Concrete.footprint #a h s
+
+let invariant #a h (s: state a) =
+  if model then
+    let s: B.pointer bytes = snd #(G.hide a) s in
+    B.live h s /\ S.length (B.deref h s) < pow2 61
+  else
+    Concrete.invariant #a h s
+
+let invariant_loc_in_footprint #_ _ _ = ()
+
+let hashed #a h (s: state a) =
+  if model then
+    let s: B.pointer bytes = snd #(G.hide a) s in
+    B.deref h s
+  else
+    let s: Concrete.state a = s in
+    Concrete.hashed h s
+
+#push-options "--max_ifuel 1"
+let hash_fits #_ _ _ =
+  assert_norm (pow2 61 < pow2 125);
+  ()
+#pop-options
+
+let frame_invariant #_ _ _ _ _ = ()
+let frame_hashed #_ _ _ _ _ = ()
+let frame_freeable #_ _ _ _ _ = ()
+
+
+/// Actual API
+/// ----------
 
 let create_in a r =
   if model then
